typing.v
@@ -1,106 +1,108 @@
 From WR Require Import syntax join.
-From Coq Require Import ssreflect.
+From Coq Require Vectors.Vector.
+From Coq Require Import Logic.StrictProp.
+Module V := Vectors.Vector.
 
-Definition context := nat -> tm.
+Notation "[[ ]]" := (nil _) (format "[[ ]]").
+Notation "h ::: t" := (V.cons _ h _ t) (at level 60, right associativity).
 
-Definition dep_ith (Γ : context) (x : fin) :=
-  ren_tm (Nat.add (S x)) (Γ x).
+Definition context n := V.t tm n.
 
-Lemma dep_ith_ren_tm (Γ : context) (A : tm) (x : fin) :
-  dep_ith (A .: Γ) (S x) = ren_tm shift (dep_ith Γ x).
-Proof.
-  case : x => [|x].
-  - rewrite /dep_ith; asimpl.
-    reflexivity.
-  - rewrite /dep_ith.
-    asimpl.
-    f_equal.
-Qed.
+Definition dep_ith {n x : fin} (Γ : context n) (p : Squash (x < n)) : tm.
+  generalize dependent x.
+  induction Γ as [|q ? ? rec].
+  - intros x p.
+    apply sEmpty_rect.
+    inversion p as [p0].
+    apply False_sind.
+    apply PeanoNat.Nat.nlt_0_r in p0.
+    assumption.
+  - destruct x as [|x].
+    + intros ?. exact (ren_tm shift q).
+    + intros p.
+      apply (ren_tm shift).
+      apply rec with (x := x).
+      inversion p as [p0].
+      apply Arith_prebase.lt_S_n in p0.
+      exact (squash p0).
+Defined.
 
-Lemma dep_ith_ren_tm0 (Γ : context) (A : tm) :
-  dep_ith (A .: Γ) 0 = ren_tm shift A.
-Proof.
-  by rewrite /dep_ith; asimpl.
-Qed.
+(* Lemma dep_ith_ren_tm {n x} (Γ : context n) (A : tm)  (p : x < n) : *)
+(*   dep_ith (V.cons _ A _ Γ) (squash (le_n_S _ _ p)) = ren_tm shift (dep_ith Γ (squash p)). *)
+(* Proof. *)
+(*   reflexivity. *)
+(* Qed. *)
+
+(* Lemma dep_ith_ren_tm0 {x n} (Γ : context n) (p : Squash (x < n)) (A : tm) : *)
+(*   dep_ith (V.cons _ A _ Γ) 0 = ren_tm shift A. *)
+(* Proof. *)
+(*   by rewrite /dep_ith; asimpl. *)
+(* Qed. *)
 
 #[export]Hint Unfold dep_ith : core.
 
-Tactic Notation "asimpldep" := repeat (progress ((try (rewrite dep_ith_ren_tm));rewrite /dep_ith; asimpl)).
+(* Tactic Notation "asimpldep" := repeat (progress ((try (rewrite dep_ith_ren_tm));rewrite /dep_ith; asimpl)). *)
 
-Inductive Wt (n : nat) (Γ : context) : tm -> tm -> Prop :=
-| T_Var i :
-  Wff n Γ ->
-  i < n ->
+Inductive Wt {n} (Γ : context n) : tm -> tm -> Prop :=
+| T_Var i (h : i < n) :
+  (* Wff Γ -> *)
   (* ------ *)
-  Wt n Γ (var_tm i) (dep_ith Γ i)
+  Wt Γ (var_tm i) (dep_ith Γ (squash h))
 
 | T_False i :
-  Wff n Γ ->
+  (* Wff Γ -> *)
   (* -------- *)
-  Wt n Γ tFalse (tUniv i)
+  Wt Γ tFalse (tUniv i)
 
 | T_Pi i A B :
-  Wt n Γ A (tUniv i) ->
-  Wt (S n) (A .: Γ) B (tUniv i) ->
+  Wt Γ A (tUniv i) ->
+  Wt (A ::: Γ) B (tUniv i) ->
   (* --------------------- *)
-  Wt n Γ (tPi A B) (tUniv i)
+  Wt Γ (tPi A B) (tUniv i)
 
 | T_Abs A a B i :
-  Wt n Γ (tPi A B) (tUniv i) ->
-  Wt (S n) (A .: Γ) a B ->
+  Wt Γ (tPi A B) (tUniv i) ->
+  Wt (A ::: Γ) a B ->
   (* -------------------- *)
-  Wt n Γ (tAbs A a) (tPi A B)
+  Wt Γ (tAbs A a) (tPi A B)
 
 | T_App a A B b :
-  Wt n Γ a (tPi A B) ->
-  Wt n Γ b A ->
+  Wt Γ a (tPi A B) ->
+  Wt Γ b A ->
   (* -------------------- *)
-  Wt n Γ (tApp a b) (subst_tm (b..) B)
+  Wt Γ (tApp a b) (subst_tm (b..) B)
 
 | T_Conv a A B i :
-  Wt n Γ a A ->
-  Wt n Γ B (tUniv i) ->
+  Wt Γ a A ->
+  Wt Γ B (tUniv i) ->
   Join A B ->
   (* ----------- *)
-  Wt n Γ a B
+  Wt Γ a B
 
 | T_On :
-  Wff n Γ ->
+  (* Wff Γ -> *)
   (* --------- *)
-  Wt n Γ tOn tSwitch
+  Wt Γ tOn tSwitch
 
 | T_Off :
-  Wff n Γ ->
+  (* Wff n Γ -> *)
   (* --------- *)
-  Wt n Γ tOff tSwitch
+  Wt Γ tOff tSwitch
 
 | T_If a b c A :
-  Wt n Γ a tSwitch ->
-  Wt n Γ b A ->
-  Wt n Γ c A ->
+  Wt Γ a tSwitch ->
+  Wt Γ b A ->
+  Wt Γ c A ->
   (* ------------ *)
-  Wt n Γ (tIf a b c) A
+  Wt Γ (tIf a b c) A
 
 | T_Switch i :
-  Wff n Γ ->
+  (* Wff Γ -> *)
   (* ----------- *)
-  Wt n Γ tSwitch (tUniv i)
+  Wt Γ tSwitch (tUniv i)
 
 | T_Univ i j :
-  Wff n Γ ->
+  (* Wff n Γ -> *)
   i < j ->
   (* ------------ *)
-  Wt n Γ (tUniv i) (tUniv j)
-
-with Wff (n : nat) (Γ : context) : Prop :=
-(* The arithmetic is needed because of the types in the context are scoped differently *)
-(* Need to skolemize the existential as F because otherwise the IH is unusable *)
-| Wff_intro F :
-  (forall i, i < n -> Wt (n - S i) (Nat.add (S i) >> Γ) (Γ i) (tUniv (F i))) ->
-  (* ---------------------------------------------------------------- *)
-  Wff n Γ.
-
-Scheme wt_ind := Induction for Wt Sort Prop
-    with wff_ind := Induction for Wff Sort Prop.
-
-Combined Scheme wt_mutual from wt_ind, wff_ind.
+  Wt Γ (tUniv i) (tUniv j).
